examples/n_german/pad.thy
@@ -1,0 +1,576 @@
+(*proof(induct_tac e and f)
+  fix x
+  show "?Pe (IVar x) s"
+  proof(case_tac "x")
+    fix x1
+    assume a1:"x=Ident x1"
+    show "?Pe (IVar x) s"
+    proof(case_tac "EX n. (  (s (Ident x1))=(index n) )\<and> n>M")
+      assume b1:"\<exists>n.  (s (Ident x1)) = index n \<and> M < n "
+      show "?Pe (IVar x) s"
+        by(cut_tac a1 b1 ,auto)
+    next
+      assume b1:"\<not>(\<exists>n.  (s (Ident x1)) = index n \<and> M < n )"
+      show "?Pe (IVar x) s"
+      proof(cut_tac  a1 b1, case_tac "(s (Ident x1))",auto)qed
+    qed
+  next
+  fix x21 x22
+    assume a1:"x = Para x21 x22"
+    show "?Pe (IVar x) s"
+    proof(case_tac "x22 >M")
+      assume b1:"x22>M "
+      show "?Pe (IVar x) s"
+        by(cut_tac a b1 a1,auto)
+    next
+      assume b1:"~x22>M "
+      show "?Pe (IVar x) s"
+      proof(case_tac "EX n. (  (s x)=(index n) )\<and> n>M",cut_tac a b1 a1,force)
+        assume c1:"\<nexists>n. s x = index n \<and> M < n"
+        have c2:" expEval (absTransfExp M (IVar x)) (abs1 M s) =s (Para x21 x22)"
+        proof(cut_tac a b1 a1 c1,case_tac "s (Para x21 x22)",auto)qed
+        have c3:"absTransfConst M (expEval (IVar x) s)=s (Para x21 x22)"
+          apply(cut_tac a b1 a1 c1,case_tac "s x",auto) done
+        show "?Pe (IVar x) s"
+          using c3 local.a1 by auto 
+      qed
+    qed
+  next
+    assume a1:"x=dontCareVar"
+    show "?Pe (IVar x) s"
+      by (simp add: a1)
+
+  qed
+next
+  fix c
+  show "?Pe (Const c) s"   
+  proof(case_tac c,auto)qed
+next
+  fix b e1 e2
+  assume a1:"?Pe e1 s" and a2:"?Pe e2 s"
+  and a3:"?Pf b s"
+  show "?Pe (iteForm b e1 e2) s"
+  
+  proof(rule impI)+
+    assume b1:"isBoundExp s i M (iteForm b e1 e2)" and b2:" M < i" 
+    let ?Q="\<lambda>s e. absTransfExp M e = dontCareExp \<or>
+    expEval (absTransfExp M e) (abs1 M s) =
+     absTransfConst M (expEval e s)"
+    let ?R="\<lambda>s f.(absTransfForm  M f=dontCareForm |
+  formEval f s =formEval (absTransfForm  M f) (abs1 M s))"
+    have b4:"isBoundFormula s i M b\<and> b\<noteq>dontCareForm"
+      using b1 isBoundExp.simps(4) isBoundFormula.simps(7) by blast
+    have b5:"isBoundExp s i M e1\<and> e1\<noteq>dontCareExp"
+      using b1 isBoundExp.simps(3) isBoundExp.simps(4) by blast 
+    have b6:"isBoundExp s i M e2\<and> e2\<noteq>dontCareExp"
+      using b1 isBoundExp.simps(3) isBoundExp.simps(4) by blast 
+    have b7:"?Q s e1"
+      using b2 b5 local.a1 by blast
+    have b8:"?Q s e2"
+      using a2 b2 b6 by blast 
+    have b9:"?R s b"
+      using a3 b2 b4 by blast
+    show "?Q s  (iteForm b e1 e2)"
+      using a3 absTransfExp.simps(3) b2 b4 b7 b8 evalITE expType.distinct(11) by presburger
+    
+  qed
+next
+  show "?Pe (dontCareExp) s"
+    by auto
+next 
+  fix e1 e2 
+  assume a1:"?Pe e1 s"  and a2:"?Pe e2 s" 
+  show "?Pf (eqn e1 e2) s"
+  proof(rule impI)+
+  assume b1:"i>M" and
+    b0:"isBoundFormula s i M (eqn e1 e2) " 
+  have b2:"isBoundExp s i M e1\<and> e1\<noteq>dontCareExp"
+    using b0 isBoundExp.simps(3) isBoundFormula.simps(1) by blast
+  have b3:"isBoundExp s i M e2\<and> e2\<noteq>dontCareExp"
+    using b0 isBoundExp.simps(3) isBoundFormula.simps(1) by blast
+  let ?Q="\<lambda>s e. absTransfExp M e = dontCareExp \<or>
+    expEval (absTransfExp M e) (abs1 M s) =
+     absTransfConst M (expEval e s)"
+  have b4:"?Q s e1"
+    using b1 b2 local.a1 by blast 
+  have b5:"?Q s e2"
+    using a2 b1 b3 by blast
+  have b6:   "absTransfForm M (eqn e1 e2) = dontCareForm \<or>
+    formEval (eqn e1 e2) s = formEval (absTransfForm M (eqn e1 e2)) (abs1 M s)"  
+    proof-       
+      have c2:"isBoolVal s e1 \<or> isEnumVal s e1 \<or> isIndexVal s e1 \<or>isDontCareVal s e1"
+        apply(unfold isBoolVal_def isEnumVal_def isIndexVal_def  typeOf_def  getValueType_def)
+        apply(cut_tac b2 ,case_tac "expEval  e1 s",auto)
+        done 
+      moreover
+      {assume c2:"isBoolVal s e1"
+        have c3:"isBoolVal s e2"
+          using b0 c2 by auto  
+        have c4:"absTransfConst M (expEval e1 s) = (expEval e1 s)"
+          using c2 boolExpEvalAbs by auto
+        have c5:"absTransfConst M (expEval e2 s) = (expEval e2 s)"
+          using c3 boolExpEvalAbs by auto
+        have "absTransfForm M (eqn e1 e2) = dontCareForm \<or>
+    formEval (eqn e1 e2) s = formEval (absTransfForm M (eqn e1 e2)) (abs1 M s)"
+          apply (simp add: a2 b1 b2 b3 c4 c5 local.a1)
+          using b4 b5 c4 c5 by auto
+         
+        
+      }  
+
+      moreover
+      {assume c2:"isEnumVal s e1"
+        have c3:"isEnumVal s e2"
+           using b0 c2 by auto    
+        have c4:"absTransfConst M (expEval e1 s) = (expEval e1 s)"
+          using c2 enumExpEvalAbs by auto
+        have c5:"absTransfConst M (expEval e2 s) = (expEval e2 s)"
+          using c3 enumExpEvalAbs by auto
+        have "absTransfForm M (eqn e1 e2) = dontCareForm \<or>
+    formEval (eqn e1 e2) s = formEval (absTransfForm M (eqn e1 e2)) (abs1 M s)"
+          apply (simp add: b4 b5 c4 c5)
+          using b4 b5 c4 c5 by auto
+         
+      }  
+      moreover
+      {assume c2:"isIndexVal s e1"
+        have c3:"isIndexVal s e2"
+          using b0 c2 by auto
+        have c4:"(the (scalar2Nat (expEval e1 s))\<le>M \<or> the (scalar2Nat (expEval e2 s))\<le>M)"
+          using b0 c2 isBoundFormula.simps(1) by blast
+        moreover
+        {assume c4:"the (scalar2Nat (expEval e1 s))\<le>M "
+        have c5:"absTransfConst M (expEval e1 s) = (expEval e1 s)  "
+          using c2 c4 indexExpEvalAbsLe by auto 
+        have c6:"absTransfForm M (eqn e1 e2) = dontCareForm \<or>
+    formEval (eqn e1 e2) s = formEval (absTransfForm M (eqn e1 e2)) (abs1 M s)"
+          apply(cut_tac b0 c2,auto)
+          using b4 b5 apply auto[1]
+          using b4 b5 c5 indexExpEvalAbsInv apply fastforce
+          using b4 b5 apply auto[1]
+          using b4 b5 c5 indexExpEvalAbsLe by auto 
+      }  
+      moreover
+        {assume c4:"the (scalar2Nat (expEval e2 s))\<le>M "
+        have c5:"absTransfConst M (expEval e2 s) = (expEval e2 s)  "
+          using c3 c4 indexExpEvalAbsLe by auto  
+        have "absTransfForm M (eqn e1 e2) = dontCareForm \<or>
+        formEval (eqn e1 e2) s = formEval (absTransfForm M (eqn e1 e2)) (abs1 M s)"
+          using b4 b5 c2 c4 c5 indexExpEvalAbsInv by auto
+          
+         
+      }  
+      ultimately  have "absTransfForm M (eqn e1 e2) = dontCareForm \<or>
+    formEval (eqn e1 e2) s = formEval (absTransfForm M (eqn e1 e2)) (abs1 M s)"
+        by blast
+    }
+   moreover
+   {assume c2:"isDontCareVal s e1"
+     have c3:"isDontCareVal s e2"
+       using b0 c2 by auto
+     have c6:"absTransfForm M (eqn e1 e2) = dontCareForm \<or>
+    formEval (eqn e1 e2) s = formEval (absTransfForm M (eqn e1 e2)) (abs1 M s)"*)
+(*       using b4 b5 c3 dontCareExpEvalAbsGe apply auto
+proof -
+  assume a1: "dontCare = absTransfConst M (expEval e1 s)"
+  assume a2: "getValueType (expEval e2 s) = ''any''"
+  assume a3: "\<And>e1 s M. getValueType (expEval e1 s) = ''any'' \<longrightarrow> absTransfConst M (expEval e1 s) = dontCare"
+  have f4: "CHR ''n'' \<noteq> CHR ''a''"
+    by simp
+  have f5: "\<forall>s. (\<exists>cs csa. s = enum cs csa) \<or> (\<exists>n. s = index n) \<or> (\<exists>b. s = boolV b) \<or> s = dontCare"
+    by (meson scalrValueType.exhaust)
+  obtain bb :: "scalrValueType \<Rightarrow> bool" where
+    f6: "\<forall>x0. (\<exists>v1. x0 = boolV v1) = (x0 = boolV (bb x0))"
+    by moura
+  obtain ccs :: "scalrValueType \<Rightarrow> char list" and ccsa :: "scalrValueType \<Rightarrow> char list" where
+    "\<forall>x0. (\<exists>v1 v2. x0 = enum v1 v2) = (x0 = enum (ccs x0) (ccsa x0))"
+by moura
+  then obtain nn :: "scalrValueType \<Rightarrow> nat" where
+    f7: "\<forall>s. s = enum (ccs s) (ccsa s) \<or> s = index (nn s) \<or> s = boolV (bb s) \<or> s = dontCare"
+    using f6 f5 by moura
+  have "absTransfConst M (expEval e2 s) = dontCare"
+    using a3 a2 by presburger
+  then show "expEval e1 s = expEval e2 s"
+    using f7 f4 a2 a1 by (metis (no_types) absTransfConst.simps(1) absTransfConst.simps(3) b0 getValueType.simps(2) isBoundFormula.simps(1) list.inject sameType_def typeOf_def)
+qed 
+*)
+(*sorry
+     }
+  ultimately  
+    show  "absTransfForm M (eqn e1 e2) = dontCareForm \<or>
+    formEval (eqn e1 e2) s = formEval (absTransfForm M (eqn e1 e2)) (abs1 M s)"
+    by blast
+
+   
+qed
+  then show  "absTransfForm M (eqn e1 e2) = dontCareForm \<or>
+    formEval (eqn e1 e2) s = formEval (absTransfForm M (eqn e1 e2)) (abs1 M s)"
+    by blast
+qed
+next
+  fix f1 f2
+  assume a1:"?Pf f1 s" and a2:"?Pf f2 s"
+  show "?Pf (andForm f1 f2) s"
+    apply(cut_tac a1 a2 ,auto)
+  qed
+
+next 
+  fix f
+  assume a1:"?Pf f s" 
+  
+   show "?Pf (neg f) s"
+   proof(rule impI)+
+     assume b1:"isBoundFormula s i M (neg f)" and b2:"i \<le>M"
+     have b3:"isBoundFormula s i M f"
+       using b1 isBoundFormula.simps(2) by blast
+     let ?R="\<lambda>s f.(absTransfForm  M f\<noteq>dontCareForm \<and>
+    absTransfForm M f \<noteq> eqn (Const (index (Suc M))) (Const (index (Suc M))) \<and>
+      formEval f s =formEval (absTransfForm  M f) (abs1 M s))"  
+     have b4:"?R s f"
+       using b2 b3 isBoundFormula.simps(7) local.a1 by blast
+     
+      
+     show "?R s (neg f)"
+      by (cut_tac b3 b4,auto) 
+      
+  qed
+
+next
+  fix f1 f2
+  assume a1:"?Pf f1 s" and a2:"?Pf f2 s"
+  show "?Pf (orForm f1 f2) s"
+  proof(cut_tac a1 a2 ,auto)
+  qed
+
+
+next
+  fix f1 f2
+  assume a1:"?Pf f1 s" and a2:"?Pf f2 s"
+  show "?Pf (implyForm f1 f2) s"
+    by(cut_tac a1 a2 ,auto)
+qed(auto)
+ 
+
+lemma absBoundExpForm:
+  assumes a:"s dontCareVar =dontCare"  
+  shows "(isBoundExp s i M e \<longrightarrow>i\<le>M\<longrightarrow>(absTransfExp  M e\<noteq>dontCareExp\<and>
+  expEval (absTransfExp  M e) (abs1 M s)  =absTransfConst M (expEval e s))) \<and>
+  (isBoundFormula s i M f \<longrightarrow>i\<le>M\<longrightarrow>(absTransfForm  M f\<noteq>dontCareForm \<and>
+   absTransfForm  M f\<noteq>eqn (Const (index (Suc M))) (Const (index (Suc M))) \<and>
+  formEval f s =formEval (absTransfForm  M f) (abs1 M s)))"
+   (is "?Pe e s \<and>   ?Pf f s") 
+proof(induct_tac e and f)
+  fix x
+  show "?Pe (IVar x) s"
+  proof(case_tac "x")
+    fix x1
+    assume a1:"x=Ident x1"
+    show "?Pe (IVar x) s"
+    proof(case_tac "EX n. (  (s (Ident x1))=(index n) )\<and> n>M")
+      assume b1:"\<exists>n.  (s (Ident x1)) = index n \<and> M < n "
+      show "?Pe (IVar x) s"
+        by(cut_tac a1 b1 ,auto)
+    next
+      assume b1:"\<not>(\<exists>n.  (s (Ident x1)) = index n \<and> M < n )"
+      show "?Pe (IVar x) s"
+      proof(cut_tac  a1 b1, case_tac "(s (Ident x1))",auto)qed
+    qed
+  next
+  fix x21 x22
+    assume a1:"x = Para x21 x22"
+    show "?Pe (IVar x) s"
+    proof(case_tac "x22 >M")
+      assume b1:"x22>M "
+      show "?Pe (IVar x) s"
+        by(cut_tac a b1 a1,auto)
+    next
+      assume b1:"~x22>M "
+      show "?Pe (IVar x) s"
+      proof(case_tac "EX n. (  (s x)=(index n) )\<and> n>M",cut_tac a b1 a1,force)
+        assume c1:"\<nexists>n. s x = index n \<and> M < n"
+        have c2:" expEval (absTransfExp M (IVar x)) (abs1 M s) =s (Para x21 x22)"
+        proof(cut_tac a b1 a1 c1,case_tac "s (Para x21 x22)",auto)qed
+        have c3:"absTransfConst M (expEval (IVar x) s)=s (Para x21 x22)"
+          apply(cut_tac a b1 a1 c1,case_tac "s x",auto) done
+        show "?Pe (IVar x) s"
+          using c3 local.a1 by auto 
+      qed
+    qed
+  next
+    assume a1:"x=dontCareVar"
+    show "?Pe (IVar x) s"
+      by (simp add: a1)
+
+  qed
+next
+  fix c
+  show "?Pe (Const c) s"   
+  proof(case_tac c,auto)qed
+next
+  fix b e1 e2
+  assume a1:"?Pe e1 s" and a2:"?Pe e2 s"
+  and a3:"?Pf b s"
+  show "?Pe (iteForm b e1 e2) s"
+  
+  proof(rule impI)+
+    assume b1:"isBoundExp s i M (iteForm b e1 e2)" and b2:"i\<le>M" 
+    let ?Q="\<lambda>s e. absTransfExp M e \<noteq> dontCareExp \<and>
+    expEval (absTransfExp M e) (abs1 M s) = absTransfConst M (expEval e s)"
+    let ?R="\<lambda>s f.(absTransfForm  M f\<noteq>dontCareForm \<and>
+  formEval f s =formEval (absTransfForm  M f) (abs1 M s))"
+    have b4:"isBoundFormula s i M b\<and> b\<noteq>dontCareForm"
+      using b1 isBoundExp.simps(4) isBoundFormula.simps(7) by blast
+    have b5:"isBoundExp s i M e1\<and> e1\<noteq>dontCareExp"
+      using b1 isBoundExp.simps(3) isBoundExp.simps(4) by blast 
+    have b6:"isBoundExp s i M e2\<and> e2\<noteq>dontCareExp"
+      using b1 isBoundExp.simps(3) isBoundExp.simps(4) by blast 
+    have b7:"?Q s e1"
+      using b2 b5 local.a1 by blast
+    have b8:"?Q s e2"
+      using a2 b2 b6 by blast 
+    have b9:"?R s b"
+      using a3 b2 b4 by blast
+    show "?Q s  (iteForm b e1 e2)"
+      using a3 absTransfExp.simps(3) b2 b4 b7 b8 evalITE expType.distinct(11) by presburger
+    
+  qed
+next
+  show "?Pe (dontCareExp) s"
+    by auto
+next 
+  fix e1 e2 
+  assume a1:"?Pe e1 s"  and a2:"?Pe e2 s" 
+  show "?Pf (eqn e1 e2) s"
+  proof(rule impI)+
+  assume b1:"i\<le>M" and
+    b0:"isBoundFormula s i M (eqn e1 e2) " 
+  have b2:"isBoundExp s i M e1\<and> e1\<noteq>dontCareExp"
+    using b0 isBoundExp.simps(3) isBoundFormula.simps(1) by blast
+  have b3:"isBoundExp s i M e2\<and> e2\<noteq>dontCareExp"
+    using b0 isBoundExp.simps(3) isBoundFormula.simps(1) by blast
+  let ?Q="\<lambda>s e. absTransfExp M e \<noteq> dontCareExp \<and>
+    expEval (absTransfExp M e) (abs1 M s) = absTransfConst M (expEval e s)"
+  have b4:"?Q s e1"
+    using b1 b2 local.a1 by blast 
+  have b5:"?Q s e2"
+    using a2 b1 b3 by blast
+  have b6:   "absTransfForm M (eqn e1 e2) \<noteq> dontCareForm \<and>
+    absTransfForm M (eqn e1 e2) \<noteq> eqn (Const (index (Suc M))) (Const (index (Suc M))) \<and>
+    formEval (eqn e1 e2) s = formEval (absTransfForm M (eqn e1 e2)) (abs1 M s)"  
+    proof-       
+      have c2:"isBoolVal s e1 \<or> isEnumVal s e1 \<or> isIndexVal s e1 \<or>isDontCareVal s e1"
+        apply(unfold isBoolVal_def isEnumVal_def isIndexVal_def  typeOf_def  getValueType_def)
+        apply(cut_tac b2 ,case_tac "expEval  e1 s",auto)
+        done 
+      moreover
+      {assume c2:"isBoolVal s e1"
+        have c3:"isBoolVal s e2"
+          using b0 c2 by auto  
+        have c4:"absTransfConst M (expEval e1 s) = (expEval e1 s)"
+          using c2 boolExpEvalAbs by auto
+        have c5:"absTransfConst M (expEval e2 s) = (expEval e2 s)"
+          using c3 boolExpEvalAbs by auto
+        have "absTransfForm M (eqn e1 e2) \<noteq> dontCareForm \<and>
+    absTransfForm M (eqn e1 e2) \<noteq> eqn (Const (index (Suc M))) (Const (index (Suc M))) \<and>
+    formEval (eqn e1 e2) s = formEval (absTransfForm M (eqn e1 e2)) (abs1 M s)"
+          apply (simp add: a2 b1 b2 b3 c4 c5 local.a1)
+        proof -
+          have "CHR ''n'' \<noteq> CHR ''b''"
+            by force
+          then show "absTransfExp M e1 = Const (index (Suc M)) \<longrightarrow> 
+        absTransfExp M e2 \<noteq> Const (index (Suc M))"
+            by (metis (no_types) b4 c2 c4 evalConst getValueType.simps(2) isBoolVal_def list.inject typeOf_def)
+        qed 
+        
+      }  
+
+      moreover
+      {assume c2:"isEnumVal s e1"
+        have c3:"isEnumVal s e2"
+           using b0 c2 by auto    
+        have c4:"absTransfConst M (expEval e1 s) = (expEval e1 s)"
+          using c2 enumExpEvalAbs by auto
+        have c5:"absTransfConst M (expEval e2 s) = (expEval e2 s)"
+          using c3 enumExpEvalAbs by auto
+        have "absTransfForm M (eqn e1 e2) \<noteq> dontCareForm \<and>
+    absTransfForm M (eqn e1 e2) \<noteq> eqn (Const (index (Suc M))) (Const (index (Suc M))) \<and>formEval (eqn e1 e2) s = formEval (absTransfForm M (eqn e1 e2)) (abs1 M s)"
+          apply (simp add: b4 b5 c4 c5)
+        proof -
+          have "''nat'' \<noteq> typeOf s e1"
+            using c2 by auto
+          then show "absTransfExp M e1 = Const (index (Suc M)) \<longrightarrow>
+           absTransfExp M e2 \<noteq> Const (index (Suc M))"
+            by (metis (no_types) b4 c4 evalConst getValueType.simps(2) typeOf_def)
+        qed 
+      }  
+      moreover
+      {assume c2:"isIndexVal s e1"
+        have c3:"isIndexVal s e2"
+          using b0 c2 by auto
+        have c4:"(the (scalar2Nat (expEval e1 s))\<le>M \<or> the (scalar2Nat (expEval e2 s))\<le>M)"
+          using b0 c2 isBoundFormula.simps(1) by blast
+        moreover
+        {assume c4:"the (scalar2Nat (expEval e1 s))\<le>M "
+        have c5:"absTransfConst M (expEval e1 s) = (expEval e1 s)  "
+          using c2 c4 indexExpEvalAbsLe by auto 
+        have c6:"absTransfForm M (eqn e1 e2) \<noteq> dontCareForm \<and>
+          absTransfForm M (eqn e1 e2) \<noteq> eqn (Const (index (Suc M))) (Const (index (Suc M)))"
+          apply(cut_tac b0 c2,auto)
+          using b4 apply blast
+          using b5 apply blast
+          apply (metis b4 c5 eq_iff evalConst not_less_eq_eq option.sel scalar2Nat.simps(1))
+          using b4 apply blast
+          using b5 apply blast
+          by (metis Suc_n_not_le_n b4 c4 c5 evalConst option.sel scalar2Nat.simps(1))  
+        have "formEval (eqn e1 e2) s = formEval (absTransfForm M (eqn e1 e2)) (abs1 M s)"
+        proof
+          assume c1:"formEval (eqn e1 e2) s "
+          show "formEval (absTransfForm M (eqn e1 e2)) (abs1 M s)"
+            using b4 b5 c1 by auto 
+          
+        next
+          assume d1:"formEval (absTransfForm M (eqn e1 e2)) (abs1 M s) "
+          have d2:"(absTransfForm M (eqn e1 e2)) =eqn (absTransfExp M (e1)) (absTransfExp M (e2))"
+            by (simp add: b4 b5) 
+          have c3:"expEval (absTransfExp M (e1)) (abs1 M s) = expEval (absTransfExp M (e2)) (abs1 M s)"
+            using d1 d2 by auto
+          have c4:"the (scalar2Nat (expEval (absTransfExp M (e2)) (abs1 M s))) \<le> M"
+            using b4 c3 c4 c5 by auto 
+          
+            
+          have c5:"expEval e2 s=(expEval (absTransfExp M (e2)) (abs1 M s))  "
+            using b0 b5 c2 c4 indexExpEvalAbsInv by auto 
+           
+          show " formEval (eqn e1 e2) s"
+            using b4 c2 c3 c4 c5 indexExpEvalAbsInv by auto 
+             
+        qed 
+
+        with c6 have "absTransfForm M (eqn e1 e2) \<noteq> dontCareForm \<and>
+      absTransfForm M (eqn e1 e2) \<noteq> eqn (Const (index (Suc M))) (Const (index (Suc M))) \<and>
+      formEval (eqn e1 e2) s = formEval (absTransfForm M (eqn e1 e2)) (abs1 M s)"
+          by blast
+      }  
+      moreover
+        {assume c4:"the (scalar2Nat (expEval e2 s))\<le>M "
+        have c5:"absTransfConst M (expEval e2 s) = (expEval e2 s)  "
+          using c3 c4 indexExpEvalAbsLe by auto 
+        have c6:"absTransfForm M (eqn e1 e2) \<noteq> dontCareForm \<and>
+          absTransfForm M (eqn e1 e2) \<noteq> eqn (Const (index (Suc M))) (Const (index (Suc M)))"
+          sorry
+        have "formEval (eqn e1 e2) s = formEval (absTransfForm M (eqn e1 e2)) (abs1 M s)"
+        proof
+          assume d1:"formEval (eqn e1 e2) s "
+          show "formEval (absTransfForm M (eqn e1 e2)) (abs1 M s)"
+            using c4 calculation(2) d1 by auto 
+          
+        next
+          assume d1:"formEval (absTransfForm M (eqn e1 e2)) (abs1 M s) "
+          have d2:"(absTransfForm M (eqn e1 e2)) =eqn (absTransfExp M (e1)) (absTransfExp M (e2))"
+            by (simp add: b4 b5) 
+          have c3:"expEval (absTransfExp M (e1)) (abs1 M s) = expEval (absTransfExp M (e2)) (abs1 M s)"
+            using d1 d2 by auto
+          have c4:"the (scalar2Nat (expEval (absTransfExp M (e1)) (abs1 M s))) \<le> M"
+            by (simp add: b5 c3 c4 c5) 
+          have c5:"expEval e1 s=(expEval (absTransfExp M (e1)) (abs1 M s))  "
+            using b4 c2 c4 indexExpEvalAbsInv by auto
+            
+          show " formEval (eqn e1 e2) s"
+            using c4 c5 calculation(2) d1 by auto 
+        qed    
+
+        with c6 have "absTransfForm M (eqn e1 e2) \<noteq> dontCareForm \<and>
+          absTransfForm M (eqn e1 e2) \<noteq> eqn (Const (index (Suc M))) (Const (index (Suc M)))
+          \<and>formEval (eqn e1 e2) s = formEval (absTransfForm M (eqn e1 e2)) (abs1 M s)"
+          by blast
+      }  
+      ultimately  have "absTransfForm M (eqn e1 e2) \<noteq> dontCareForm \<and>
+          absTransfForm M (eqn e1 e2) \<noteq> eqn (Const (index (Suc M))) (Const (index (Suc M)))
+          \<and>formEval (eqn e1 e2) s = formEval (absTransfForm M (eqn e1 e2)) (abs1 M s)"
+        by blast
+    }
+   moreover
+   {assume c2:"isDontCareVal s e1"
+     have c3:"isDontCareVal s e2"
+       using b0 c2 by auto
+     have c6:"absTransfForm M (eqn e1 e2) \<noteq> dontCareForm \<and>
+          absTransfForm M (eqn e1 e2) \<noteq> eqn (Const (index (Suc M))) (Const (index (Suc M)))"
+       using b4 b5 c3 dontCareExpEvalAbsGe by auto 
+     have "formEval (eqn e1 e2) s = formEval (absTransfForm M (eqn e1 e2)) (abs1 M s)" 
+       apply(cut_tac c2,auto)
+       using b4 apply blast
+       using b5 apply blast
+       apply (simp add: b4 b5)+
+     proof -
+       assume a1: "getValueType (expEval e1 s) = ''any''"
+       have "\<forall>n. getValueType (index n) \<noteq> getValueType dontCare"
+         by simp
+       then show "expEval e1 s = expEval e2 s"
+         using a1 by (metis absTransfConst.simps(1) absTransfConst.simps(3) c3 dontCareExpEvalAbsGe getValueType.simps(4) isDontCareVal_def scalrValueType.exhaust typeOf_def)
+     qed
+     
+    with c6 have "absTransfForm M (eqn e1 e2) \<noteq> dontCareForm \<and>
+          absTransfForm M (eqn e1 e2) \<noteq> eqn (Const (index (Suc M))) (Const (index (Suc M)))
+          \<and>formEval (eqn e1 e2) s = formEval (absTransfForm M (eqn e1 e2)) (abs1 M s)"
+        by blast  
+     }
+  ultimately  have "absTransfForm M (eqn e1 e2) \<noteq> dontCareForm \<and>
+          absTransfForm M (eqn e1 e2) \<noteq> eqn (Const (index (Suc M))) (Const (index (Suc M)))
+          \<and>formEval (eqn e1 e2) s = formEval (absTransfForm M (eqn e1 e2)) (abs1 M s)"
+    by blast
+
+  then show "absTransfForm M (eqn e1 e2) \<noteq> dontCareForm \<and>
+    absTransfForm M (eqn e1 e2) \<noteq> eqn (Const (index (Suc M))) (Const (index (Suc M))) \<and>
+    formEval (eqn e1 e2) s = formEval (absTransfForm M (eqn e1 e2)) (abs1 M s)"
+    by blast
+    
+    qed
+    show "absTransfForm M (eqn e1 e2) \<noteq> dontCareForm \<and>
+    absTransfForm M (eqn e1 e2) \<noteq> eqn (Const (index (Suc M))) (Const (index (Suc M))) \<and>
+    formEval (eqn e1 e2) s = formEval (absTransfForm M (eqn e1 e2)) (abs1 M s) "
+    using b4 b5 b6 apply auto
+    done
+qed
+
+next
+  fix f1 f2
+  assume a1:"?Pf f1 s" and a2:"?Pf f2 s"
+  show "?Pf (andForm f1 f2) s"
+  proof(cut_tac a1 a2 ,auto)
+  qed
+
+next 
+  fix f
+  assume a1:"?Pf f s" 
+  
+   show "?Pf (neg f) s"
+   proof(rule impI)+
+     assume b1:"isBoundFormula s i M (neg f)" and b2:"i \<le>M"
+     have b3:"isBoundFormula s i M f"
+       using b1 isBoundFormula.simps(2) by blast
+     let ?R="\<lambda>s f.(absTransfForm  M f\<noteq>dontCareForm \<and>
+    absTransfForm M f \<noteq> eqn (Const (index (Suc M))) (Const (index (Suc M))) \<and>
+      formEval f s =formEval (absTransfForm  M f) (abs1 M s))"  
+     have b4:"?R s f"
+       using b2 b3 isBoundFormula.simps(7) local.a1 by blast
+     
+      
+     show "?R s (neg f)"
+      by (cut_tac b3 b4,auto) 
+      
+  qed
+
+next
+  fix f1 f2
+  assume a1:"?Pf f1 s" and a2:"?Pf f2 s"
+  show "?Pf (orForm f1 f2) s"
+  proof(cut_tac a1 a2 ,auto)
+  qed
+
+
+next
+  fix f1 f2
+  assume a1:"?Pf f1 s" and a2:"?Pf f2 s"
+  show "?Pf (implyForm f1 f2) s"
+    by(cut_tac a1 a2 ,auto)
+qed(auto)
